Cannon example

cannon/CannonA.v
@@ -2,44 +2,32 @@ Require Import CRIS.
 Require Import ImpPrelude.
 Require Import CannonHeader.
 
-Set Implicit Arguments.
+Local Definition RA := excl_authR unitO.
 
-Section RA.
-  Context `{!crisG Γ Σ α β τ _S _I}.
-  
-  Local Definition RA := excl_authR unitO.
+Class cannonGpreS `{!crisG Γ Σ α β τ _S _I} := {
+  #[local] cannon_inG :: inG (excl_authR unitO) Γ;
+}.
+Class cannonGS `{!crisG Γ Σ α β τ _S _I} := {
+  #[local] cannonGS_cannonGpreS :: cannonGpreS;
+  cannon_name : gname;
+}.
+Definition cannonΓ : HRA := #[excl_authR unitO].
+Global Instance subG_cannonGpreS `{!crisG Γ Σ α β τ _S _I} : subG cannonΓ Γ → cannonGpreS.
+Proof. solve_inG. Defined.
 
-  Class cannonG `{!crisG Γ Σ α β τ _S _I} := {
-    cannon_inG :: inG (excl_authR unitO) Γ;
-  }.
-  Definition cannonΓ : HRA := #[excl_authR unitO].
-  Global Instance subG_cannonG : subG cannonΓ Γ → cannonG.
-  Proof. solve_inG. Defined.
-End RA.
-Hint Unfold subG_cannonG cannon_inG : GRA_index.
+Module CannonA. Section CannonA.
+  Context `{!crisG Γ Σ α β τ _S _I, !concGS, !cannonGS}.
 
-Module CannonAS. Section CannonAS.
-  Context `{!crisG Γ Σ α β τ _S _I}.
-  Context `{!cannonG}.
-                   
-  Definition Ready : iProp Σ := own base_γ (●E tt).
-  Definition Ball : iProp Σ := own base_γ (◯E tt).
-  Definition Fired : iProp Σ := own base_γ ((●E tt) ⋅ (◯E tt)).
-
-  Definition ir : DRA_mk RA := ●E tt ⋅ ◯E tt.
-  Lemma ir_valid : ✓ ir. Proof. rewrite /ir. eapply excl_auth_valid. Qed.
-  Definition irΓ : cannonΓ := *[Some ir].
+  Definition Ready : iProp Σ := own cannon_name (●E tt).
+  Definition Ball : iProp Σ := own cannon_name (◯E tt).
+  Definition Fired : iProp Σ := own cannon_name ((●E tt) ⋅ (◯E tt)).
 
   Lemma ReadyBall : Ready ∗ Ball ⊣⊢ Fired.
-  Proof.
-    rewrite /Ready /Ball /Fired. iSplit.
-    { iIntros "[B W]". iSplitL "B"; iFrame. }
-    { iIntros "[$ $]". }
-  Qed.
+  Proof. rewrite /Ready /Ball /Fired own_op //. Qed.
 
   Lemma FiredReady : Ready ∗ Fired ⊢ False.
   Proof.
-    rewrite /Ready /Fired. iIntros "[B0 [B1 W]]". iCombine "B0 B1" as "X" gives %FALSE.
+    rewrite /Ready /Fired; iIntros "[B0 [B1 W]]". iCombine "B0 B1" as "X" gives %FALSE.
     rewrite excl_auth_auth_op_valid // in FALSE.
   Qed.
 
@@ -52,20 +40,10 @@ Module CannonAS. Section CannonAS.
   Definition fire_spec : fspec :=
     fspec_simple (λ _ : unit,
       ((λ arg, (⌜arg = ([]: list val)↑⌝ ∗ Ball)),
-      (λ ret, (⌜ret = (1: Z)%Z↑⌝)))
+       (λ ret, (⌜ret = (1: Z)%Z↑⌝)))
     )%I.
 
-  Definition Sp : spl_type :=
-    Seal.sealing CRIS [(Some CannonHdr.fire, fsp_some fire_spec)].
-
-  Lemma Sp_nodup : List.NoDup (List.map fst Sp).
-  Proof. unfold Sp. unseal CRIS. prove_nodup. Qed.
-End CannonAS. End CannonAS.
-
-Module CannonA. Section CannonA.
-  Import CannonAS.
-  Context `{!crisG Γ Σ α β τ _S _I}.
-  Context `{!cannonG}.
+  Definition sp : specmap := {[speckey_fn CannonHdr.fire := fspec_to_rel fire_spec]}.
 
   Definition scopes := ["Cannon"].
   Definition v_lv := "Cannon" ↯ "lv".
@@ -76,18 +54,23 @@ Module CannonA. Section CannonA.
       _ <- trigger (@IO _ unit "print" [r]↑);;
       Ret r.
 
-  Definition fnsems : fnsems_type :=
-    [(Some CannonHdr.fire, (true, wmask_all, scopes, (fsp_some CannonAS.fire_spec, cfunU fire)))].
+  Definition fnsems : fnsemmap :=
+    {[Some CannonHdr.fire := Some (msk_scp scopes msk_true, (fsp_some fire_spec, cfunU fire))]}.
 
   Program Definition smod : SMod.t := {|
     SMod.scopes := scopes;
     SMod.fnsems := fnsems;
-    SMod.initial_st := [(v_lv, 1%Z↑)];
+    SMod.initial_st := ∅;
   |}.
-  Solve All Obligations with prove_scope.
-  Next Obligation. prove_nodup. Qed.
+  Solve All Obligations with mod_tac.
 
-  Definition init_cond : iProp Σ := Ready.
-
-  Definition t sp := Seal.sealing CRIS (SMod.to_mod sp smod).
+  Definition t sp := SMod.to_mod sp smod.
 End CannonA. End CannonA.
+
+Lemma cannon_alloc `{!crisG Γ Σ α β τ _S _I, !cannonGpreS} :
+  ⊢ o=> ∃ (_ : cannonGS), CannonA.Ready ∗ CannonA.Ball.
+Proof.
+  iMod (own_alloc (●E tt ⋅ ◯E tt)) as "[%c [? ?]]".
+  { apply : excl_auth_valid. }
+  by iExists (Build_cannonGS _ _ _ _ _ _ _ _ _ c); iFrame.
+Qed.
