cannon/CannonAll.v
@@ -4,46 +4,37 @@ Require Import CannonHeader CannonI CannonMainI.
 Require Import CannonA CannonMainA.
 Require Import CannonIAproof CannonMainIAproof.
 
-Module CannonAll.
-  Import inv_instances.
-  Local Instance Γ : HRA := ##[invΓ; cannonΓ].
-  Local Instance Σ : GRA := ##[Γ; invΣ].
-  Local Definition irΓ : Γ := **[ir_invΓ; CannonAS.irΓ].
-  Local Definition irΣ : Σ := **[irΓ; ir_invΣ].
-
-  Local Lemma irΣ_valid : ✓ (irΣ ⋅ ir_own_admin).
-  Proof.
-    solve_ir_valid.
-    - apply CannonAS.ir_valid.
-  Qed.
-
+Section CannonAux.
+  Import CannonA.
+  Context `{!crisG Γ Σ α β τ Hsub Hinv, !concGS, !cannonGS}.
   Local Definition smod_src : SMod.t := CannonA.smod ☆ (MainA.smod 1).
-  Local Definition mod_top : Mod.t := (SMod.to_mod sp_none (SMod.cancel smod_src)).
+  Local Definition mod_top : Mod.t := (SMod.to_mod ∅ (SMod.cancel smod_src)).
   Local Definition mod_tgt : Mod.t := CannonI.t ★ (MainI.t 1).
   
-  Local Definition sp : sp_type := sp_from smod_src.
+  Local Definition sp : specmap := SMod.conc_sp_from smod_src.
   Local Definition mod_src : Mod.t := SMod.to_mod sp smod_src.
 
-  Local Definition init_cond : iProp Σ :=
-    winv (⊤, ⊤) ∗ CannonA.init_cond ∗ MainA.init_cond.
-
-  (* Apply cancellation to linked spec module *)
   Lemma cancel_src :
-    refines (mod_top, init_cond)
-            (mod_src, init_cond).
+    refines (mod_top, Ready ∗ TID 0 ∗ YIELD 0 ∗ winv (⊤, ⊤) ∗ Ball ∗ TIDAUTH 0 ∗ YIELDAUTH 1)%I
+            (mod_src, Ready)%I.
   Proof.
     eapply Cancel.cancellation.
-    - ii; des; subst; inv FIND; ss; rewrite !eq_rel_dec_correct in H0; des_ifs.
-    - econs; [refl|]; i; inv NS; des; inv H; des; inv H1;
-      rewrite !eq_rel_dec_correct in H2; des_ifs.
-    - econs; unfold_mod; ss; prove_nodup.
+    { apply SMod.cancellable_add; r; rewrite /=; mod_tac ss. }
+    { assert (Ht : SMod.conc_sp_from smod_src !! speckey_entry =
+        fsp_some (MainA.main_spec)); last (rewrite Ht; clear Ht).
+      { rewrite lookup_insert_ne // lookup_kmap_Some; exists None; split; ss. }
+       eexists _, _; splits.
+      { ss; exists (tt); split; refl. }
+      { iIntros "[? [? [? $]]]"; ss. }
+      { unfold_pre_post. iIntros "% % %"; by des. }
+    }
   Qed.
 
   (* Refinement between spec/impl of whole program (linked module) *)
-  Lemma src_tgt : refines (mod_src, init_cond) (mod_tgt, emp%I).
+  Lemma src_tgt : refines (mod_src, Ready) (mod_tgt, emp%I).
   Proof.
     eapply ctxr_refines.
-    rewrite /mod_src /mod_tgt /smod_src add_interp_comm.
+    rewrite /mod_src /mod_tgt /smod_src SMod.to_mod_add.
 
     etrans; cycle 1.
     { ctxr_rotate. ctxr_drop. eapply CannonIA.ctxr. }
@@ -51,19 +42,15 @@ Module CannonAll.
     etrans; cycle 1.
     { ctxr_rotate. ctxr_drop. eapply CannonMainIA.ctxr.
       instantiate (1:=sp).
-      rewrite /CannonAS.Sp. unseal CRIS. econs; first prove_nodup.
-      ii. inv H. des_ifs.
-      unfold dec, option_Dec, AList.option_Dec_obligation_1 in Heq.
-      des_ifs.
+      repeat try eapply insert_subseteq_l; last apply map_empty_subseteq;
+        rewrite lookup_insert_ne // lookup_kmap_Some; eexists (Some _); split; ss.
     }
 
-    rewrite /CannonA.t /MainA.t /init_cond. unseal CRIS. 
-    eapply ctxr_cond_strengthen.
-    iIntros "[? [? ?]]". iFrame.
+    eapply ctxr_cond_strengthen. by iIntros "$".
   (*SLOW*)Qed.
 
   Lemma top_tgt :
-    refines (mod_top, init_cond)
+    refines (mod_top, Ready ∗ TID 0 ∗ YIELD 0 ∗ winv (⊤, ⊤) ∗ Ball ∗ TIDAUTH 0 ∗ YIELDAUTH 1)%I
             (mod_tgt, emp%I).
   Proof.
     etrans.
@@ -71,34 +58,43 @@ Module CannonAll.
     { eapply src_tgt. }
   Qed.
 
-  Lemma tgt_wf:
-    Mod.wf mod_tgt.
+  Lemma tgt_wf : Mod.wf mod_tgt.
   Proof.
-    rewrite /mod_tgt /CannonI.t /MainI.t; unseal CRIS; prove_nodup.
+    eapply Mod.add_wf.
+    { econs; eauto; [mod_tac|prove_nodup]. }
+    { econs; eauto; [mod_tac|prove_nodup]. }
+    { set_solver. }
+    { prove_nodup; set_solver. }
   Qed.
+End CannonAux.
 
-  Lemma init_cond_valid:
-    ∃ rs, ✓ rs ∧ (Own rs ⊢ |==> init_cond).
-  Proof.
-    exists (irΣ ⋅ ir_own_admin). split.
-    - apply irΣ_valid.
-    - simplify_res.
-      { rewrite make_own_admin; iFrame.
-        iDestruct "H12" as "[? ?]". iFrame. et.
-      }
-      all: solve_res.
-  Qed.
+Module CannonAll.
+  Import inv_instances.
+  Local Instance Γ : HRA := ##[invΓ; concΓ; cannonΓ].
+  Local Instance Σ : GRA := ##[Γ; invΣ].
 
   Theorem behavioral_refinement :
-    ∃ src_res tgt_res, refines_lmod
+    ∃ β τ (Hinv : invGS Γ Σ α) (_ : crisG Γ Σ α β τ _ Hinv) (_ : concGS) (_ : cannonGS)
+      src_res tgt_res,
+      refines_lmod
       (Mod.to_lmod mod_top src_res)
       (Mod.to_lmod mod_tgt tgt_res).
   Proof.
-    move: (top_tgt)=>H; rewrite /refines in H; des; ss.
-    hexploit H; eauto using tgt_wf. clear H; intros [WF H].
-    assert (IV:= init_cond_valid). des.
-    destruct (H rs); des; et.
-    rewrite IV0 /init_cond {1}winv_split_empty. iIntros ">[[? ?] ?]". iFrame. et.
+    apply own_admin_soundness.
+    iMod winv_alloc as "[% [% [% [% ?]]]]"; iExists _, _, _, _.
+    iMod conc_alloc as "[% ?]"; iExists _.
+    iMod cannon_alloc as "[% [? ?]]"; iExists _.
+    pose proof top_tgt as Href.
+    iStopProof. eapply entails_pointwise; iIntros (res Hres) "R".
+    iPoseProof (Own_valid with "R") as "%".
+    rewrite /refines in Href; hexploit Href; eauto using tgt_wf.
+    clear Href; intros [? Href].
+    iPureIntro; hexploit (Href res); eauto.
+    { rewrite Hres; iIntros "[W [[$ [$ [$ $]]] [$ $]]]".
+      rewrite {1}winv_split_empty comm //.
+    }
+    intros [rt ?].
+    exists res, rt; by des.
   Qed.
 (*SLOW*)End CannonAll.
 (* Print Assumptions CannonAll.behavioral_refinement. *)
