cannon/CannonI.v
@@ -2,12 +2,8 @@ Require Import CRIS.
 Require Import ImpPrelude.
 Require Import CannonHeader.
 
-Set Implicit Arguments.
-
 Module CannonI. Section CannonI.
-  Local Open Scope string_scope.
-
-  Context `{Σ: GRA}.
+  Context `{!crisG Γ Σ α β τ _S _I, !concGS}.
 
   Definition scopes := ["Cannon"].
   Definition v_lv := "Cannon" ↯ "lv". (* local variable *)
@@ -15,7 +11,7 @@ Module CannonI. Section CannonI.
   Definition div (n m : Z) : option Z :=
     if Z_zerop m then None else Some (Z.div n m).
 
-  Definition fire: list val -> itree crisE Z :=
+  Definition fire : list val → itree crisE Z :=
     λ _,
       powder <- cgetU v_lv;;
       r <- (div 1 powder)?;;
@@ -23,16 +19,15 @@ Module CannonI. Section CannonI.
       cput v_lv (powder - 1)%Z;;;
       Ret r.
 
-  Definition fnsems : fnsems_type :=
-    [(Some CannonHdr.fire, (false, wmask_all, scopes, (None, cfunU fire)))].
+  Definition fnsems : fnsemmap :=
+    {[Some CannonHdr.fire := Some (msk_scp scopes msk_true, (None, cfunU fire))]}.
   
   Program Definition smod : SMod.t := {|
     SMod.scopes := scopes;
     SMod.fnsems := fnsems;
-    SMod.initial_st := [(v_lv, 1%Z↑)];
+    SMod.initial_st := {[v_lv := Some 1%Z↑]};
   |}.
-  Solve All Obligations with prove_scope.
-  Next Obligation. prove_nodup. Qed.
+  Solve All Obligations with mod_tac.
 
-  Definition t := Seal.sealing CRIS (SMod.to_mod sp_none smod).
+  Definition t := SMod.to_mod ∅ smod.
 End CannonI. End CannonI.
