cannon/CannonIAproof.v
@@ -2,62 +2,51 @@ Require Import CRIS.
 Require Import ImpPrelude.
 Require Import CannonHeader CannonI CannonA.
 
-Set Implicit Arguments.
-Local Open Scope nat_scope.
-
 Module CannonIA. Section CannonIA.
-  Import CannonAS.
-  Context `{!crisG Γ Σ α β τ _S _I}.
-  Context `{!cannonG}.
+  Context `{!crisG Γ Σ α β τ _S _I, !concGS, !cannonGS}.
+  Import CannonA.
 
-  Context (Sp_s : sp_type).
+  Context (sp : specmap).
 
-  Definition Ist : alist key Any.t → alist key Any.t → iProp Σ :=
-    (λ st_s st_t,
-      (⌜st_s = [(CannonA.v_lv, 1%Z↑)] /\ st_t = [(CannonI.v_lv, 1%Z↑)]⌝ ∗ Ready)
-      ∨ Fired
-    )%I.
+  Definition Ist : ist_type Σ :=
+    (λ st_s st_t, (⌜st_t = {[CannonI.v_lv := Some 1%Z↑]}⌝ ∗ Ready) ∨ Fired)%I.
   
-  Local Definition CannonAMod := (CannonA.t Sp_s).
+  Local Definition CannonAMod := (CannonA.t sp).
   Local Definition CannonIMod := (CannonI.t).
 
-  Lemma simF_fire : ISim.sim_fun open CannonAMod CannonIMod CannonA.init_cond Ist (Some CannonHdr.fire).
+  Lemma simF_fire : ISim.sim_fun open CannonAMod CannonIMod Ist (Some CannonHdr.fire).
   Proof using.
-    init_simF.
+    iStartSim.
 
     (* SRC: precondition *)
-    steps_l. iDestruct "ASM" as "(%Q & (%Y & B))". subst. hss.
-    unfold Ist. iDestruct "IST" as "[[% R] | F]"; des; subst; cycle 1. 
+    steps_l. iDestruct "ASM" as "(-> & -> & B)". hss.
+    iDestruct "IST" as "[[% R] | F]"; des; subst; cycle 1. 
     (* already fired *)
-    { iExFalso. iApply FiredBall. iFrame. }
+    { iExFalso. iApply FiredBall; iFrame. }
 
-    steps_r. hss. steps_r.
+    steps_l. steps_r. hss. steps_r.
     change (1 `div` 1)%Z with 1%Z.
-    
+
     (* SRC, TGT: print 1 *)
     step. steps_r.
 
     (* prove postcondition & the IST - Ready * Ball = Shot *)
-    rewrite /alist_upd /_alist_upd /=. replace (1 - 1)%Z with 0%Z by nia.
     steps_l. forces_l. iSplitR; eauto. step.
     iSplit; eauto. iRight. iApply ReadyBall; iFrame.
   (*SLOW*)Qed.
 
-  Theorem sim : ISim.t open CannonAMod CannonIMod CannonA.init_cond Ist.
+  Lemma sim : ISim.t open CannonAMod CannonIMod CannonA.Ready Ist.
   Proof using.
     init_sim.
-    - split; eauto. iIntros "IC". unfold Ist, CannonA.init_cond. iLeft. iFrame; eauto.
+    - iIntros "IC"; iLeft; iFrame; eauto.
     - eapply simF_fire.
   Qed.
 End CannonIA.
 
 Section ctxr.
-  Context `{!crisG Γ Σ α β τ _S _I}.
-  Context `{!cannonG}.
+  Context `{!crisG Γ Σ α β τ _S _I, !concGS, !cannonGS}.
 
-  Theorem ctxr (Sp_s : sp_type):
-    ctx_refines
-      (CannonA.t Sp_s, CannonA.init_cond)
-      (CannonI.t, emp%I).
+  Lemma ctxr (sp : specmap) :
+    ctx_refines (CannonA.t sp, CannonA.Ready) (CannonI.t, emp%I).
   Proof using. eapply main_adequacy, sim. Qed.
 End ctxr. End CannonIA.
